Basic A1 check.

eve/Src/Delivery/studio/tools/autoproof/base_theory.bpl
@@ -120,8 +120,16 @@ function in_domain(h: HeapType, o: ref, o': ref): bool
 	)
 }
 
-axiom (forall h: HeapType, o, o': ref :: { in_domain(h, o, o') } h[o, closed] && h[o, owns][o'] ==> in_domain(h, o, o'));
-axiom (forall h: HeapType, o, o': ref :: { in_domain(h, o, o') } o != o' && Set#Equal(Set#Empty(), h[o, owns]) ==> !in_domain(h, o, o'));
+axiom (forall h: HeapType, o, o': ref :: { in_domain(h, o, o') } IsHeap(h) && h[o, closed] && h[o, owns][o'] ==> in_domain(h, o, o'));
+axiom (forall h: HeapType, o, o': ref :: { in_domain(h, o, o') } IsHeap(h) && o != o' && Set#Equal(Set#Empty(), h[o, owns]) ==> !in_domain(h, o, o'));
+
+// Is o' in the transitive owns of o?
+// (the same as in_domain if o is closed)
+function trans_owns(h: HeapType, o: ref, o': ref): bool
+{
+  o == o' || h[o, owns][o'] || (exists x: ref :: h[o, owns][x] && trans_owns(h, x, o'))
+}
+
 
 // ----------------------------------------------------------------------
 // Frames
@@ -172,7 +180,17 @@ const readable: Frame;
 // Is invariant of object o satisifed?
 function user_inv(h: HeapType, o: ref): bool;
 
-// Reads axiom
+// Read frame of user_inv
+function user_inv_readable(HeapType, ref): Frame;
+axiom (forall<T> h: HeapType, x: ref, o: ref, f: Field T :: { user_inv_readable(h, x)[o, f] }
+  IsHeap(h) ==> user_inv_readable(h, x)[o, f] == (trans_owns(h, x, o) || h[x, subjects][o]));
+  
+// // Part of read frame of user_inv closed under domains (used for function calls)
+// function user_inv_function_readable(HeapType, ref): Frame;
+// axiom (forall<T> h: HeapType, x: ref, o: ref, f: Field T :: { user_inv_function_readable(h, x)[o, f] }
+  // IsHeap(h) ==> user_inv_function_readable(h, x)[o, f] == trans_owns(h, x, o));  
+
+// Frame axiom
 axiom (forall h, h': HeapType, x: ref :: { user_inv(h', x), HeapSucc(h, h') } 
   IsHeap(h) && IsHeap(h') && HeapSucc(h, h') &&
   x != Void && h[x, allocated] && h'[x, allocated] &&   
