eve/Src/framework/eiffel2boogie/tests/framing/ownership/observer_inheritance/f_oi_observer.e
@@ -49,9 +49,9 @@ feature {F_OI_SUBJECT} -- Internal communication
 
 invariant
 	subject_exists: subject /= Void
+	subjects_structure: subjects = [subject]
 	subject_aware: subject.observers.has (Current)
 	synchronized: is_synchronized (subject.value)
-	subjects_structure: subjects = [subject]
 	subject_not_in_domain: not domain_has (subject)
 	observers_structure: observers.is_empty
 end
