eve/Src/framework/eiffel2boogie/tests/framing/ownership/observer_one_to_many/f_oom_subject_d.e
@@ -91,9 +91,9 @@ feature {F_OOM_OBSERVER_D} -- Internal communication
 
 invariant
 	subscribers_exists: subscribers /= Void
+	owns_structure: owns = [subscribers]
 	all_subscribers_exist: across subscribers.sequence as o all attached o.item end
 	observers_structure: observers = subscribers.sequence.range
-	owns_structure: owns = [subscribers]
 	subjects_structure: subjects = []
 
 end
